ETCSFinite.sml
@@ -1,0 +1,656 @@
+
+
+
+(*
+
+val bvs = List.map (dest_var o rastt) ["a:1->A","s:1->Exp(A,1+1)"] 
+val t = rastt "Ins(a:1->A,s:1->Exp(A,1+1))"
+
+
+val bvs = List.map (dest_var o rastt) ["n:1->N","m:1->N"] 
+val t = rastt "Sub(n:1->N,m)"
+val (f,s,tl) = dest_fun t
+
+
+
+
+fn finfo =>  binop_t "o" (corres_fterm finfo [])
+Binarymap.peek(!fsym2IL,"Ins")
+
+corres_fterm finfo (List.map mk_var bvs
+
+val f = “IN(a:1->A,f:Exp(A,1+1)->Exp(A,1+1) o s:1->Exp(A,1+1))”
+val (P,tl) = dest_pred f
+val p = rastt "In(A)";
+val l = List.map (dest_var o rastt) ["a:X->A","ss:X->Exp(A,1+1)"]
+
+
+qform2IL [‘s:1-> Exp(Exp(X,1+1),1+1)’] ‘!a.IN(a:1->Exp(X,1+1),f o s) ==> IN(a,s)’
+
+
+pain point of form2IL
+*)
+
+
+
+
+(*
+qform2IL [‘a:1->A’,‘s:1-> Exp(A,1+1)’] ‘IN(a:1->A,s)’
+
+val bvs = List.map (dest_var o rastt) ["a:1->A","s:1->Exp(A,1+1)"] 
+val f = “IN(a:1->A,s)”
+val (P,tl) = dest_pred f
+val p = rastt "In(A)";
+val l = List.map (dest_var o rastt) ["a:1->A","ss:1->Exp(A,1+1)"]
+
+
+‘!a:1->A.IN(a, f o s) ==> IN(a,s)’
+
+ rw[SS_def] >> strip_tac >>
+ strip_tac >>
+ qexists_tac 
+ ‘ALL(Imp(In(A) o Pa(p1(A,Exp(A,1+1)), f o p2(A,Exp(A,1+1))),In(A)))’ >>
+*)  
+
+val prim_lemma = prove_store("SS_lemma",
+e0
+cheat
+(form_goal
+“!A f:Exp(A,1+1)->Exp(A,1+1). ?!p:Exp(A,1+1) ->1+1.
+  !a.p o a = TRUE <=> SS(f o a,a)”));
+
+
+val prim_lemma' = prove_store("SS_lemma'",
+e0
+cheat
+(form_goal
+“!A f:Exp(A,1+1)->Exp(A,1+1). ?!p:1-> Exp(Exp(A,1+1),1+1).
+  !a.IN(a,p)<=> SS(f o a,a)”));
+
+use "ETCSreln.sml";
+(* the pred used in FI's_def is 
+   \a.FIs(X) o a ⊆ a*)
+(*Rel2Ar is the thing corresponds to P2fun*)
+
+val _ = new_fsym2IL("Fst",(rastt "p1(A,B)",[dest_var (rastt "ab:X->A * B")]));
+val _ = new_fsym2IL("Snd",(rastt "p2(A,B)",[dest_var (rastt "ab:X->A * B")]));
+
+val _ = new_fsym2IL("Snd",(rastt "p2(A,B)",[dest_var (rastt "ab:X->A * B")]));
+
+
+val IN_Tp1 = prove_store("IN_Tp1",
+e0
+(rw[IN_def,In_def,Tp1_def,Ev_of_Tp_el',o_assoc,p12_of_Pa,idR])
+(form_goal “!A a:1->A s.IN(a,Tp1(s)) <=> s o a = TRUE”));
+
+local
+val FI_cl = 
+ “(xs = Empty(X) ==> IN(xs,FIs)) &
+  (!xs0 x:1->X. IN(xs0,FIs) & xs = Ins(x,xs0) ==> IN(xs,FIs))”
+in
+val (FI_incond,x1) = mk_incond FI_cl;
+val FIr_def = define_fsym("FIr",[("X",ob_sort)]) (qform2IL [‘a : 1->Exp(Exp(X,1+1),1+1)’,‘a' : 1->Exp(Exp(X,1+1),1+1)’]
+ ‘!xs. IN(xs,a') <=> 
+       (xs = Empty(X) |
+       ?xs0  x:1->X.
+        IN(xs0, a) & xs = Ins(x, xs0))’)
+val IL_lemma = 
+proved_th $
+e0
+(rpt strip_tac  >>
+ rw[o_assoc,Pa_distr,DISJ_def,p12_of_Pa,Eq_property_TRUE,
+             one_to_one_id,idR,FIr_def] >>
+ rw[Ex_def,o_assoc] >> rw[CONJ_def,Pa_distr] >>
+ rw[p31_def,p32_def,p33_def] >>
+ once_rw[p52_def] >> once_rw[p51_def] >> once_rw[p53_def] >>
+ once_rw[p54_def] >> once_rw[p55_def] >> 
+ once_rw[All_def] >> rw[o_assoc,IFF_def,Pa_distr] >>
+ rw[DISJ_def,o_assoc,Pa_distr] >>
+ rw[Ex_def,o_assoc] >> rw[CONJ_def,Pa_distr] >>
+ rw[o_assoc,p12_of_Pa,Pa_distr] >>
+ rw[one_to_one_id] >> rw[idR,Eq_property_TRUE] >>
+ rw[IN_def,Ins_def])
+(form_goal “!a:1->Exp(Exp(X,1+1),1+1) a'.
+ FIr(X) o Pa(a,a') =TRUE <=>
+  (!xs. IN(xs,a') <=> 
+       (xs = Empty(X) |
+       ?xs0  x:1->X.
+        IN(xs0, a) & xs = Ins(x, xs0)))”);
+(* given a: 1-> Exp(Exp(X,1+1),1+1)
+    want a': 1-> Exp(Exp(X,1+1),1+1), which is an arrow:
+   Exp(X,2) -> 2,saying that "is" in the set a', then its transpose is the set 
+   a'*)
+val FIsi_def = 
+define_fsym("FIsi",[dest_var (rastt "a : 1->Exp(Exp(X,1+1),1+1)")]) (qform2IL [‘xs : 1->Exp(X,2)’]
+ ‘xs = Empty(X) |
+          ?xs0  x:1->X.
+            IN(xs0, a) & xs = Ins(x, xs0)’);
+val FIsi_property = proved_th $
+e0
+(rw[FIsi_def] >> rpt strip_tac >>
+ rw[o_assoc,DISJ_def,Pa_distr] >> 
+ once_rw[Ex_def] >> rw[o_assoc,Ex_def] >>
+ rw[CONJ_def,Pa_distr,o_assoc] >>
+ rw[one_to_one_id,idR] >>
+ once_rw[p31_def,p32_def,p33_def] >>
+ rw[p12_of_Pa,o_assoc,Pa_distr] >>
+ rw[Eq_property_TRUE,IN_def,Ins_def,idL])
+(form_goal 
+“!a: 1->Exp(Exp(X,1+1),1+1) xs. FIsi(a) o xs = TRUE <=>
+ xs = Empty(X) |
+          ?xs0  x:1->X.
+            IN(xs0, a) & xs = Ins(x, xs0) ”);
+val FIf_precond = proved_th $
+e0
+(strip_tac >>
+ qsuff_tac
+ ‘?a'.
+ (!xs. IN(xs,a') <=> 
+       (xs = Empty(X) |
+       ?xs0  x:1->X.
+        IN(xs0, a) & xs = Ins(x, xs0)))’ 
+ >-- (strip_tac >> uex_tac >> qexists_tac ‘a'’ >>
+      arw[] >> rpt strip_tac >> irule $ iffLR IN_EXT >> arw[]) >>
+ qexists_tac ‘Tp1(FIsi(a))’ >>
+ rw[IN_Tp1] >> rw[FIsi_property])
+(form_goal “!a. ?!a'.
+ (!xs. IN(xs,a') <=> 
+       (xs = Empty(X) |
+       ?xs0  x:1->X.
+        IN(xs0, a) & xs = Ins(x, xs0)))”)
+val FIf_def = 
+Rel2Ar' 
+|> sspecl [rastt "FIr(X)"]
+|> rewr_rule[IL_lemma]
+|> C mp FIf_precond
+|> qSKOLEM "FIf" [‘X’]
+|> spec_all |> qgen ‘b’
+|> qspecl [‘FIf(X) o a’]
+|> rewr_rule[] |> qgen ‘a’
+val FIf_monotone = mk_monotone FIf_def;
+val FI's_def = mk_prim FIf_def;
+val FIs_def = mk_LFP (rastt "FI's(X)");
+val FIs_cond = mk_cond FIs_def FI's_def;
+val FIs_SS = mk_SS FIs_def FI's_def;
+val FI_rules0 = mk_rules FIf_monotone FIs_SS FIs_cond;
+val FI_cases0 = mk_cases FIf_monotone FI_rules0 FIs_cond;
+val FI_ind0 = mk_ind FIs_cond;
+val FI_ind1 = mk_ind1 FIf_def FI_ind0;
+val FI_ind2 = mk_ind2 FI_ind1;
+val FI_cases1 = mk_case1 FIf_def FI_cases0;
+val FI_rules1 = mk_rules1 FIf_def FI_rules0;
+val FI_rules2 = mk_rules2 FI_rules1;
+val FI_rules3 = mk_rules3 FI_rules2;
+end
+
+val FI_ind = FI_ind2 |> store_as "FI_ind";
+val FI_cases = FI_cases1 |> store_as "FI_cases";
+val FI_rules = FI_rules3 |> store_as "FI_rules";
+
+
+
+val DEL_def = proved_th $
+e0
+(cheat)
+(form_goal “!X.?!DEL:Exp(X,1+1) * X -> Exp(X,1 + 1).
+ !x0 xs x. IN(x,DEL o Pa(xs,x0)) <=> IN(x,xs) & ~(x = x0)”)
+|> spec_all |> uex2ex_rule
+|> qSKOLEM "DEL" [‘X’]
+|> gen_all
+|> store_as "DEL_def";
+
+
+val Del_def = qdefine_fsym("Del",[‘s0:1-> Exp(X,1+1)’,‘x0:1->X’])
+‘DEL(X) o Pa(s0,x0)’ |> qgen ‘x0’ |> qgen ‘s0’ |> qgen ‘X’
+|> store_as "Del_def";
+
+
+val Ins_def1 = INS_def |> rewr_rule[GSYM Ins_def] |> store_as "Ins_def1";
+val Del_def1 = DEL_def |> rewr_rule[GSYM Del_def] |> store_as "Del_def1";
+
+
+val Del_Ins = prove_store("Del_Ins",
+e0
+(rpt strip_tac >> irule $ iffLR IN_EXT >> 
+ arw[Ins_def1,Del_def1] >>
+ rpt strip_tac >> dimp_tac >> strip_tac >> arw[] >> ccontra_tac >> fs[])
+(form_goal “!X x0:1->X xs0. (~IN(x0,xs0)) ==> Del(Ins(x0,xs0),x0) =xs0”));
+
+
+
+
+val Ins_absorb = prove_store("Ins_absorb",
+e0
+(rpt strip_tac >> irule $ iffLR IN_EXT >> rw[Ins_def1] >>
+ rpt strip_tac >> dimp_tac >> strip_tac >> arw[])
+(form_goal “!X x0:1->X xs0. IN(x0,xs0) ==> Ins(x0,xs0) =xs0”));
+
+
+val Fin_def = qdefine_psym("Fin",[‘A:1->Exp(X,1+1)’]) ‘IN(A,FIs(X))’
+                          |> gen_all |> store_as "Fin_def"; 
+
+
+
+
+local
+val Cd_cl = 
+ “(xsn = Pa(Empty(X),O) ==> IN(xsn,Cds)) &
+  (!xsn0 x. IN(xsn0,Cds) & ~(IN(x,Fst(xsn0))) & 
+            xsn = Pa(Ins(x,Fst(xsn0)),Suc(Snd(xsn0))) ==> IN(xsn,Cds))”
+in
+val (Cd_incond,x1) = mk_incond Cd_cl;
+val Cdr_def = define_fsym("Cdr",[("X",ob_sort)]) (qform2IL [‘a : 1->Exp(Exp(X,1+1) * N,1+1)’,‘a' : 1->Exp(Exp(X,1+1) * N,1+1)’]
+ ‘!xsn : 1 -> Exp(X, 1+1) * N.
+     IN(xsn, a') <=>
+     xsn = Pa(Empty(X), O) |
+     ?xsn0: 1 -> Exp(X,1+1) * N  x:1->X.
+       IN(xsn0, a) &
+       ~IN(x, Fst(xsn0)) & xsn = Pa(Ins(x, Fst(xsn0)), Suc(Snd(xsn0)))’)
+val IL_lemma = 
+proved_th $
+e0
+(rpt strip_tac  >>
+ rw[o_assoc,Pa_distr,DISJ_def,p12_of_Pa,Eq_property_TRUE,
+             one_to_one_id,idR,Cdr_def] >>
+ rw[one_to_one_id,idL,idR] >>
+ once_rw[All_def,o_assoc,Pa_distr] >>
+ rw[IFF_def,o_assoc,Pa_distr] >>
+ rw[DISJ_def,o_assoc,Pa_distr] >>
+ once_rw[Ex_def] >> rw[o_assoc] >> once_rw[Ex_def] >>
+ once_rw[o_assoc] >> once_rw[Pa_distr] >> once_rw[CONJ_def] >>
+ once_rw[o_assoc] >> once_rw[Pa_distr] >> once_rw[CONJ_def] >>
+ once_rw[p52_def] >> once_rw[p51_def] >> once_rw[p53_def] >>
+ once_rw[p54_def] >> once_rw[p55_def] >> 
+ once_rw[p31_def] >> once_rw[p32_def] >> once_rw[p33_def] >>
+ once_rw[o_assoc] >> once_rw[NEG_def'] >>
+ once_rw[Pa_distr] >> once_rw[Eq_property_TRUE] >>
+ once_rw[p12_of_Pa] >> once_rw[p12_of_Pa] >> 
+ rw[Pa_distr] >> rw[p12_of_Pa,o_assoc] >> rw[Pa_distr] >>
+ rw[p12_of_Pa] >> rw[one_to_one_id] >> rw[idR] >>
+ once_rw[o_assoc] >> once_rw[p12_of_Pa] >>
+ once_rw[o_assoc] >> once_rw[p12_of_Pa] >>
+ rw[p12_of_Pa] >>
+ rw[GSYM Fst_def,GSYM Snd_def] >>
+ rw[Ins_def,IN_def] >> rw[Suc_def])
+(form_goal “!a:1->Exp(Exp(X,1+1)* N,1+1) a'.
+ Cdr(X) o Pa(a,a') =TRUE <=>
+  (!xsn : 1 -> Exp(X, 1+1) * N.
+     IN(xsn, a') <=>
+     xsn = Pa(Empty(X), O) |
+     ?xsn0: 1 -> Exp(X,1+1) * N  x:1->X.
+       IN(xsn0, a) &
+       ~IN(x, Fst(xsn0)) & xsn = Pa(Ins(x, Fst(xsn0)), Suc(Snd(xsn0))))”);
+(* given a: 1-> Exp(Exp(X,1+1),1+1)
+    want a': 1-> Exp(Exp(X,1+1),1+1), which is an arrow:
+   Exp(X,2) -> 2,saying that "is" in the set a', then its transpose is the set 
+   a'*)
+val Cdsi_def = 
+define_fsym("Cdsi",[dest_var (rastt "a : 1->Exp(Exp(X,1+1)*N,1+1)")]) (qform2IL [‘xsn : 1->Exp(X,2) * N’]
+ ‘xsn = Pa(Empty(X), O) |
+     ?xsn0: 1 -> Exp(X,1+1) * N  x:1->X.
+       IN(xsn0, a) &
+       ~IN(x, Fst(xsn0)) & xsn = Pa(Ins(x, Fst(xsn0)), Suc(Snd(xsn0)))’);
+val Cdsi_property = proved_th $
+e0
+(rw[Cdsi_def] >> rpt strip_tac >>
+ rw[o_assoc,DISJ_def,Pa_distr] >> 
+ once_rw[Ex_def] >> rw[o_assoc,Ex_def] >>
+ rw[CONJ_def,Pa_distr,o_assoc] >>
+ rw[one_to_one_id,idR] >>
+ once_rw[p31_def,p32_def,p33_def] >>
+ rw[p12_of_Pa,o_assoc,Pa_distr] >>
+ rw[Eq_property_TRUE,IN_def,Ins_def,NEG_def'] >>
+ rw[GSYM Fst_def,GSYM Snd_def,Suc_def,idL])
+(form_goal 
+“!a: 1->Exp(Exp(X,1+1) * N,1+1) xsn. Cdsi(a) o xsn = TRUE <=>
+ xsn = Pa(Empty(X), O) |
+     ?xsn0: 1 -> Exp(X,1+1) * N  x:1->X.
+       IN(xsn0, a) &
+       ~IN(x, Fst(xsn0)) & xsn = Pa(Ins(x, Fst(xsn0)), Suc(Snd(xsn0))) ”);
+val Cdf_precond = proved_th $
+e0
+(strip_tac >>
+ qsuff_tac
+ ‘?a'.
+ !xsn. IN(xsn,a') <=> 
+       (xsn = Pa(Empty(X), O) |
+     ?xsn0: 1 -> Exp(X,1+1) * N  x:1->X.
+       IN(xsn0, a) &
+       ~IN(x, Fst(xsn0)) & xsn = Pa(Ins(x, Fst(xsn0)), Suc(Snd(xsn0))))’ 
+ >-- (strip_tac >> uex_tac >> qexists_tac ‘a'’ >>
+      arw[] >> rpt strip_tac >> irule $ iffLR IN_EXT >> arw[]) >>
+ qexists_tac ‘Tp1(Cdsi(a))’ >>
+ rw[IN_Tp1] >> rw[Cdsi_property])
+(form_goal “!a. ?!a'.
+ !xsn. IN(xsn,a') <=> 
+ (xsn = Pa(Empty(X), O) |
+     ?xsn0: 1 -> Exp(X,1+1) * N  x:1->X.
+       IN(xsn0, a) &
+       ~IN(x, Fst(xsn0)) & xsn = Pa(Ins(x, Fst(xsn0)), Suc(Snd(xsn0))))”)
+val Cdf_def = 
+Rel2Ar' 
+|> sspecl [rastt "Cdr(X)"]
+|> rewr_rule[IL_lemma]
+|> C mp Cdf_precond
+|> qSKOLEM "Cdf" [‘X’]
+|> spec_all |> qgen ‘b’
+|> qspecl [‘Cdf(X) o a’]
+|> rewr_rule[] |> qgen ‘a’;
+val Cdf_monotone = mk_monotone Cdf_def;
+val Cd's_def = mk_prim Cdf_def;
+val Cds_def = mk_LFP (rastt "Cd's(X)");
+val Cds_cond = mk_cond Cds_def Cd's_def;
+val Cds_SS = mk_SS Cds_def Cd's_def;
+val Cd_rules0 = mk_rules Cdf_monotone Cds_SS Cds_cond;
+val Cd_cases0 = mk_cases Cdf_monotone Cd_rules0 Cds_cond;
+val Cd_ind0 = mk_ind Cds_cond;
+val Cd_ind1 = mk_ind1 Cdf_def Cd_ind0;
+val Cd_ind2 = mk_ind2 Cd_ind1;
+val Cd_cases1 = mk_case1 Cdf_def Cd_cases0;
+val Cd_rules1 = mk_rules1 Cdf_def Cd_rules0;
+val Cd_rules2 = mk_rules2 Cd_rules1;
+val Cd_rules3 = mk_rules3 Cd_rules2;
+end
+
+val Cd_ind = Cd_ind2 |> store_as "Cd_ind";
+val Cd_cases = Cd_cases1 |> store_as "Cd_cases";
+val Cd_rules = Cd_rules3 |> store_as "Cd_rules";
+
+
+
+val Cds_ind = prove_store("Cds_ind",
+e0
+(rpt gen_tac >> disch_tac >>
+ qsuff_tac
+ ‘!xsn. IN(xsn,Cds(X)) ==> IN(xsn,ss)’
+ >-- (fconv_tac (depth_fconv no_conv forall_cross_fconv) >> rw[]) >>
+ match_mp_tac Cd_ind (* irule does not work *) >>
+ fconv_tac (depth_fconv no_conv forall_cross_fconv) >> 
+ rw[Pair_def'] >> arw[]
+ )
+(form_goal 
+ “!X ss.IN(Pair(Empty(X),O),ss) & 
+ (!xs0 n0 x. IN(Pair(xs0,n0),ss)  & ~(IN(x,xs0)) ==> 
+  IN(Pair(Ins(x,xs0),Suc(n0)),ss)) ==> 
+ !xs n. IN(Pair(xs,n),Cds(X)) ==> IN(Pair(xs,n),ss)”));
+
+
+val Cd_induct0 = prove_store("Cd_induct0",
+e0
+(strip_tac >>
+ x_choose_then "s" (assume_tac o conjE1) 
+ (IN_def_P_expand |> qspecl [‘Pow(X) * N’]) >>
+ arw[Cds_ind])
+(form_goal 
+ “!X.P(Pair(Empty(X),O)) & 
+ (!xs0 n0 x:mem(X). P(Pair(xs0,n0)) & ~(IN(x,xs0)) ==> 
+  P(Pair(Ins(x,xs0),Suc(n0)))) ==> 
+ !xs n. IN(Pair(xs,n),Cds(X)) ==> P(Pair(xs,n))”));
+
+
+val Cd_induct = prove_store("Cd_induct",
+e0
+(strip_tac >> assume_tac (Cd_induct0 |> qspecl [‘X’] 
+            |> fVar_sInst_th “P(xsn:mem(Pow(X) * N))”
+               “P(Fst(xsn:mem(Pow(X) * N)),Snd(xsn))”
+            |> rewr_rule[Pair_def']) >> arw[])
+(form_goal 
+ “!X.P(Empty(X),O) & 
+ (!xs0 n0 x:mem(X). P(xs0,n0) & ~(IN(x,xs0)) ==> 
+  P(Ins(x,xs0),Suc(n0))) ==> 
+ !xs n. IN(Pair(xs,n),Cds(X)) ==> P(xs,n)”));
+ 
+val Fin_induct = prove_store("Fin_induct",
+e0
+(rw[Fin_def] >> strip_tac >>
+ x_choose_then "s" (assume_tac o conjE1) 
+ (IN_def_P_expand |> qspecl [‘Pow(X)’]) >>
+ arw[FI_ind])
+(form_goal 
+ “!X.P(Empty(X)) & 
+ (!xs0:mem(Pow(X)) x. P(xs0) ==> P(Ins(x,xs0))) ==> 
+ !xs:mem(Pow(X)). Fin(xs) ==> P(xs)”));
+ 
+
+(*Card rel*)
+val Cdr_def = qdefine_psym("Cdr",[‘xs:mem(Pow(X))’,‘n:mem(N)’])
+‘IN(Pair(xs,n),Cds(X))’ |> qgenl[‘X’,‘xs’,‘n’] 
+|> store_as "Cdr_def";
+
+val Cdr_induct = Cd_induct |> rewr_rule[GSYM Cdr_def]
+                           |> store_as "Cdr_induct";
+
+
+val Cdr_Empty = prove_store("Cdr_Empty",
+e0
+(rw[Cdr_def,Cd_rules])
+(form_goal
+ “!X.Cdr(Empty(X),O)”));
+
+val Cdr_Ins = Cd_rules |> conjE2 |> spec_all |> undisch |> gen_all |> disch_all
+                       |> gen_all
+                       |> qspecl [‘X’,‘Pair(xs0:mem(Pow(X)),n:mem(N))’]
+                       |> rewr_rule[GSYM Cdr_def,Pair_def']
+                       |> gen_all
+                       |> store_as "Cdr_Ins";
+
+
+
+val Ins_NONEMPTY = prove_store("Ins_NONEMPTY",
+e0
+(rpt strip_tac >> rw[GSYM IN_EXT_iff,Ins_def,Empty_def] >>
+ ccontra_tac >> first_x_assum (qspecl_then [‘x0’] assume_tac) >> fs[])
+(form_goal
+ “!X x0 xs:mem(Pow(X)).~(Ins(x0,xs) = Empty(X))”));
+
+val IN_Ins_SND = prove_store("IN_Ins_SND",
+e0
+(rw[Ins_def] >> rpt strip_tac)
+(form_goal “!X x0 xs0:mem(Pow(X)) x. IN(x, Ins(x0, xs0)) & (~(x = x0)) ==> IN(x,xs0)”));
+
+val Cdr_Empty_unique = prove_store("Cdr_Empty_unique",
+e0
+(rw[Cdr_def] >> once_rw[Cd_cases] >> rpt strip_tac >>
+ fs[Pair_eq_eq,GSYM Ins_NONEMPTY])
+(form_goal
+ “!X n.Cdr(Empty(X),n) ==> n = O”));
+
+
+
+
+val Del_Ins_SWAP = prove_store("Del_Ins_SWAP",
+e0
+(rpt strip_tac >> rw[GSYM IN_EXT_iff,Ins_def,Del_def] >>
+ rpt strip_tac >> dimp_tac >> rpt strip_tac >> arw[])
+(form_goal
+ “!X x0 x:mem(X).(~(x0 = x)) ==> !xs.Del(Ins(x0, xs), x) = Ins(x0,Del(xs,x))”));
+
+
+val Cdr_Ins = 
+Cd_cases |> qspecl [‘Pair(Ins(x0:mem(X),xs0),n:mem(N))’]
+|> rewr_rule[Pair_eq_eq,Ins_NONEMPTY] 
+|> conv_rule (basic_fconv no_conv exists_cross_fconv)
+|> rewr_rule[Pair_def',GSYM Cdr_def]
+|> gen_all |> store_as "Cdr_Ins";
+
+val Cdr_Empty = Cd_rules |> conjE1 |> gen_all |> rewr_rule[GSYM Cdr_def] 
+                         |> store_as "Cdr_Empty";
+
+
+val Cdr_Del = prove_store("Cdr_Del",
+e0
+(strip_tac >> ind_with (Cdr_induct |> qspecl [‘X’]) >>
+ rw[Cdr_Empty,Empty_def] >> rpt strip_tac (* 2 *)
+ >-- (irule $ iffRL Cdr_Ins >>
+     qexistsl_tac [‘xs0’,‘n0’,‘x’] >> arw[]) >>
+ rw[Pre_Suc] >>
+ qcases ‘x' = x’ >> fs[] (* 2 *)
+ >-- (drule Del_Ins >> arw[]) >>
+ qby_tac ‘IN(x',xs0)’ >-- (irule IN_Ins_SND >> qexists_tac ‘x’ >> arw[]) >>
+ first_x_assum drule >> 
+ qcases ‘n0 = O’ 
+ >-- (fs[] >> qsuff_tac ‘xs0 = Empty(X)’ >-- (strip_tac >> fs[Empty_def]) >>
+      qpick_x_assum ‘Cdr(xs0, O)’ mp_tac >>
+      rw[Cdr_def] >> once_rw[Cd_cases] >> rw[Pair_eq_eq,GSYM Suc_NONZERO] >>
+      rpt strip_tac) >>
+ fs[O_xor_Suc] >> fs[Pre_Suc] >> 
+ qby_tac ‘Del(Ins(x, xs0), x') = Ins(x, Del(xs0,x'))’
+ >-- (irule Del_Ins_SWAP >> ccontra_tac >> fs[]) >>
+ arw[] >> irule $ iffRL Cdr_Ins >> 
+ qexistsl_tac [‘Del(xs0, x')’,‘pn’,‘x’] >> arw[Del_def])
+(form_goal
+ “!X xs:mem(Pow(X)) n.Cdr(xs,n) ==> 
+  Cdr(xs,n) & !x. IN(x,xs) ==> Cdr(Del(xs,x),Pre(n))”));
+
+
+val Fin_Card = prove_store("Card_Fun",
+e0
+(strip_tac >> ind_with (Fin_induct |> qspecl [‘X’]) >> rpt strip_tac (* 2 *)
+ >-- (uex_tac >> qexists_tac ‘O’ >> rw[Cdr_Empty,Cdr_Empty_unique]) >>
+ pop_assum (strip_assume_tac o uex_expand) >> uex_tac >>
+ qcases ‘IN(x,xs0)’ 
+ >-- (drule Ins_absorb >> arw[] >> qexists_tac ‘n’ >> arw[]) >>
+ qexists_tac ‘Suc(n)’ >> rpt strip_tac (* 2 *)
+ >-- (irule $ iffRL Cdr_Ins >> qexistsl_tac [‘xs0’,‘n’,‘x’] >> arw[]) >>
+ drule Cdr_Del >> fs[] >>
+ first_x_assum (qspecl_then [‘x’] assume_tac) >>
+ fs[Ins_def] >> drule Del_Ins >> fs[] >>
+ first_x_assum drule >> pop_assum (assume_tac o GSYM) >> arw[] >>
+ qsuff_tac ‘~(n' = O)’ >-- (rw[O_xor_Suc] >> strip_tac >> arw[Pre_Suc]) >>
+ rw[O_xor_Suc] >> qpick_x_assum ‘Cdr(Ins(x, xs0), n')’ mp_tac >>
+ strip_tac >> drule $ iffLR Cdr_Ins >> pop_assum strip_assume_tac >>
+ qexists_tac ‘b’ >> arw[])
+(form_goal
+ “!X xs:mem(Pow(X)).Fin(xs) ==> ?!n.Cdr(xs,n)”));
+
+val CARD_def = 
+    AX1 |> qspecl [‘Pow(X)’,‘N’] 
+        |> fVar_sInst_th “P(xs:mem(Pow(X)), n:mem(N))”
+           “(Fin(xs:mem(Pow(X))) & Cdr(xs,n)) | (~Fin(xs) & n = O)”
+        |> uex2ex_rule
+        |> qSKOLEM "CARD" [‘X’]
+        |> gen_all |> store_as "CARD_def";
+
+val CARD_unique = proved_th $
+e0
+(rpt strip_tac >> rw[CARD_def] >> 
+ qcases ‘Fin(xs)’ 
+ >-- (drule Fin_Card >> pop_assum (strip_assume_tac o uex_expand) >>
+      uex_tac >> qexists_tac ‘n’ >> arw[]) >>
+ uex_tac >> qexists_tac ‘O’ >> arw[])
+(form_goal “!X xs:mem(Pow(X)). ?!n. Holds(CARD(X),xs,n)”)
+ 
+ 
+val Cd0_def = P2fun |> qspecl [‘Pow(X)’,‘N’] 
+                 |> fVar_sInst_th “P(x:mem(Pow(X)),y:mem(N))”
+                    “Holds(CARD(X),x,y)” 
+                 |> C mp (CARD_unique |> qspecl [‘X’]) 
+                 |> qSKOLEM "Cd0" [‘X’] |> gen_all |> store_as "Cd0_def";
+
+
+val Card_def = qdefine_fsym ("Card",[‘xs:mem(Pow(X))’])
+                            ‘App(Cd0(X),xs)’
+                            |> gen_all |> store_as "Card_def";
+
+val Del_Empty = prove_store("Del_Empty",
+e0
+(rw[GSYM IN_EXT_iff,Del_def,Empty_def])
+(form_goal
+ “!X x. Del(Empty(X),x) = Empty(X)”));
+
+val Ins_eq_eq = prove_store("Ins_eq_eq",
+e0
+(rpt strip_tac >-- (ccontra_tac >>
+ qsuff_tac ‘~(IN(a2,Ins(a2,s2)))’
+ >-- rw[Ins_def] >>
+ qsuff_tac ‘~(IN(a2,Ins(a1,s1)))’
+ >-- arw[] >>
+ arw[Ins_def] >> flip_tac >> first_x_assum accept_tac) >>
+ irule IN_EXT >> strip_tac >> dimp_tac >> strip_tac (* 2 *)
+ >-- (qby_tac ‘IN(x,Ins(a1,s1))’ >-- arw[Ins_def] >> rfs[] >>
+      fs[Ins_def] >> pop_assum (assume_tac o GSYM) >> fs[]) >>
+ qpick_x_assum ‘Ins(a1, s1) = Ins(a2, s2)’ (assume_tac o GSYM) >>
+ qby_tac ‘IN(x,Ins(a2,s2))’ >-- arw[Ins_def] >>
+ rfs[] >> fs[Ins_def] >> pop_assum (assume_tac o GSYM) >> fs[])
+(form_goal
+ “!A a1:mem(A) s1 a2 s2. ~(IN(a1,s1)) & ~(IN(a2,s2)) & ~(IN(a1,s2)) & ~(IN(a2,s1)) & 
+ Ins(a1,s1) = Ins(a2,s2) ==> a1 = a2 & s1 = s2”));
+
+val Fin_Empty = FI_rules |> conjE1 |> rewr_rule[GSYM Fin_def] 
+                         |> gen_all |> store_as "Fin_Empty";
+
+val Fin_Ins = FI_rules |> conjE2 |> rewr_rule[GSYM Fin_def]
+                       |> spec_all |> undisch |> gen_all |> disch_all 
+                       |> gen_all |> store_as "Fin_Ins";
+
+val Fin_Del0 = prove_store("Fin_Del",
+e0
+(strip_tac >> ind_with (Fin_induct |> qspecl [‘X’]) >> 
+ rw[Fin_Empty,Del_Empty] >> rpt strip_tac (* 2 *)
+ >-- (drule Fin_Ins >> arw[]) >>
+ qcases ‘x = x'’ (* 2 *)
+ >-- (arw[] >> qcases ‘IN(x',xs0)’ (* 2 *)
+     >-- (drule Ins_absorb >> arw[]) >>
+     drule Del_Ins >> arw[]) >>
+ drule Del_Ins_SWAP >> arw[] >>
+ irule Fin_Ins >> arw[])
+(form_goal
+ “!X xs:mem(Pow(X)).Fin(xs) ==> Fin(xs) &  !x. Fin(Del(xs,x)) ”));
+
+val Fin_Del = prove_store("Fin_Del",
+e0
+(rpt strip_tac >> drule Fin_Del0 >> arw[])
+(form_goal “!X xs:mem(Pow(X)).Fin(xs) ==> !x. Fin(Del(xs,x))”));
+
+val Card_Fin = prove_store("Card_Fin",
+e0
+(rpt strip_tac >> arw[Card_def,Cd0_def,CARD_def])
+(form_goal
+ “!X xs:mem(Pow(X)). Fin(xs) ==>
+  (!n. Card(xs) = n <=> Cdr(xs,n))”));
+
+
+val Card_Empty = prove_store("Card_Empty",
+e0
+(strip_tac >> qspecl_then [‘X’] assume_tac Fin_Empty >>
+ drule Card_Fin >> arw[Cdr_Empty])
+(form_goal
+ “!X. Card(Empty(X)) = O”));
+
+
+val Cdr_Card = prove_store("Cdr_Card",
+e0
+(rpt strip_tac >> drule Card_Fin >>
+ pop_assum (assume_tac o GSYM) >> arw[])
+(form_goal “!X xs:mem(Pow(X)). Fin(xs) ==> 
+ Cdr(xs, Card(xs))”));
+
+
+val Card_Ins = prove_store("Card_Ins",
+e0
+(rpt strip_tac >> drule Fin_Ins >>
+ first_x_assum (qspecl_then [‘x’] assume_tac) >>
+ drule Card_Fin >> arw[] >> irule $ iffRL Cdr_Ins >>
+ qexistsl_tac [‘xs’,‘Card(xs)’,‘x’] >> arw[] >>
+ (* Cdr(xs, Card(xs))*)
+ rw[Card_def] >> 
+ qsspecl_then [‘xs’,‘App(Cd0(X), xs)’] assume_tac Cd0_def >>
+ fs[] >> fs[CARD_def])
+(form_goal
+ “!X xs:mem(Pow(X)). 
+  Fin(xs) ==> !x.~(IN(x,xs)) ==> Card(Ins(x,xs)) = Suc(Card(xs))”));
+
+
+
+val Card_Del = prove_store("Card_Del",
+e0
+(rpt strip_tac >> drule Fin_Del >> 
+ first_x_assum (qspecl_then [‘x’] assume_tac) >>
+ drule Card_Fin >> arw[] >>
+ irule (Cdr_Del |> spec_all |> undisch |> conjE2 |> disch_all |> gen_all) >>
+ arw[] >> irule Cdr_Card >> arw[])
+(form_goal
+ “!X xs:mem(Pow(X)). Fin(xs) ==> 
+  !x. IN(x,xs) ==> Card(Del(xs,x)) = Pre(Card(xs))”));
+ 
+
