ETCSreln.sml
@@ -1,0 +1,959 @@
+
+
+
+
+
+
+fun mk_App fnterm arg = mk_o fnterm arg
+
+
+fun conj_monotone ip1 ip2 = 
+    let val A2A' = concl ip1
+        val B2B' = concl ip2
+        val (A,A') = dest_imp A2A'
+        val (B,B') = dest_imp B2B'
+        val AnB = mk_conj A B
+        val A'nB' = mk_conj A' B'
+        val AnB2A' = assume AnB |> conjE1 |> mp ip1
+        val AnB2B' = assume AnB |> conjE2 |> mp ip2
+    in conjI AnB2A' AnB2B' |> disch AnB
+    end
+
+
+fun disj_monotone ip1 ip2 = 
+    let val A2A' = concl ip1
+        val B2B' = concl ip2
+        val (A,A') = dest_imp A2A'
+        val (B,B') = dest_imp B2B'
+        val AuB = mk_disj A B
+        val A'uB' = mk_disj A' B'
+        val A2A'uB' = assume A |> mp ip1 |> disjI1 B'
+        val B2A'uB' = assume B |> mp ip2 |> disjI2 A'
+    in disjE (assume AuB) A2A'uB' B2A'uB' |> disch AuB
+    end
+
+fun forall_monotone allip = 
+    let val ((n,s),ip) = allip |> concl |> dest_forall
+        val (ante,conseq) = dest_imp ip
+        val allante = mk_forall n s ante
+        val allconseq = mk_forall n s conseq 
+        val v0 = mk_var(n,s)
+    in allante |> assume |> allE v0 |> mp (allE v0 allip) |> allI (n,s)
+               |> disch allante 
+    end
+
+
+fun exists_monotone allip = 
+    let val ((n,s),ip) = allip |> concl |> dest_forall
+        val (ante,conseq) = dest_imp ip
+        val exante = mk_exists n s ante
+        val exconseq = mk_exists n s conseq 
+        val v0 = mk_var(n,s)
+    in ante |> assume |> mp (allE v0 allip) |> existsI (n,s) v0 conseq
+            |> existsE (n,s) (assume exante)
+            |> disch exante
+    end
+
+
+fun trivial_imp f = iffLR $ frefl f 
+
+
+fun imp_induce ip fm = 
+    let val ((n,s),b) = dest_forall (concl ip)
+        val v0 = mk_var (n,s)
+        val ip1 = allE v0 ip
+        val (ante0,conseq0) = dest_imp (concl ip1)
+        val (ante,conseq) = dest_imp fm
+    in (*assume ante and conseq same pattern*)
+        if eq_form(ante,conseq) then trivial_imp ante else 
+        if can (match_form essps (HOLset.empty String.compare) ante ante0) mempty
+        then let val env = match_form essps 
+                           (HOLset.empty String.compare) ante0 ante mempty
+                 val ip1' = inst_thm env ip1 
+                 val (ante',conseq') = dest_imp (concl ip1')
+             in if eq_form(ante,ante') andalso eq_form(conseq,conseq') 
+                then ip1' else 
+                raise simple_fail "imp_induce"
+             end
+        else
+        case (view_form ante,view_form conseq) of 
+            (vConn("&",[a1,a2]),vConn("&",[c1,c2])) => 
+            let val ip1 = imp_induce ip (mk_imp a1 c1)
+                val ip2 = imp_induce ip (mk_imp a2 c2)
+            in conj_monotone ip1 ip2
+            end 
+          | (vConn("|",[a1,a2]),vConn("|",[c1,c2])) => 
+            let val ip1 = imp_induce ip (mk_imp a1 c1)
+                val ip2 = imp_induce ip (mk_imp a2 c2)
+            in disj_monotone ip1 ip2
+            end 
+          (*assume the two sides has the same bound name to work!*)
+          | (vQ("!",n1,s1,b1),vQ("!",n2,s2,b2)) => 
+            let val ip0 = imp_induce ip (mk_imp b1 b2)
+            in forall_monotone (allI (n1,s1) ip0)
+            end
+          | (vQ("?",n1,s1,b1),vQ("?",n2,s2,b2)) => 
+            let val ip0 = imp_induce ip (mk_imp b1 b2)
+            in exists_monotone (allI (n1,s1) ip0)
+            end
+    end
+
+
+(*maybe have something like dest_IN which dests a particular pred*)
+fun mk_monotone fdef = 
+    let val (pvar as (pname,psort),b) = fdef |> concl |> dest_forall
+        val (mvar as (mname,msort),b1) = b |> dest_forall
+        val (b1l,b1r) = dest_dimp b1 
+        val fnterm = b1l |> dest_pred |> #2 |> el 2 |> dest_fun |> #3 |> hd
+        val avoids = cont fdef
+        val gens1 = pvariantt avoids (mk_var("s1",psort))
+        val gens2 = pvariantt avoids (mk_var("s2",psort))
+        val goalant = mk_pred "SS" [gens1,gens2] 
+        val goalconsq = mk_pred "SS" [mk_App fnterm gens1,mk_App fnterm gens2]
+        val goalant_ipth = goalant |> basic_fconv no_conv 
+                                   (rewr_fconv (spec_all SS_def))
+                                   |> iffLR |> undisch
+        val goalconsq' = goalconsq |> basic_fconv no_conv 
+                                      (first_fconv [rewr_fconv(spec_all SS_def),
+                                                 rewr_fconv (spec_all fdef)])
+        val (var0,toinduce)= goalconsq' |> concl |> #2 o dest_dimp |> dest_forall
+        val imp_induce_th = imp_induce goalant_ipth toinduce
+        val th1 = imp_induce_th |> allI var0 |> dimp_mp_r2l goalconsq'
+                                |> disch goalant 
+                                |> allI (dest_var gens2)
+                                |> allI (dest_var gens1)
+    in th1
+    end
+
+
+val IN_def_P_ex = prove_store("IN_def_P_ex",
+e0
+(cheat)
+(form_goal “!A P:A-> 1+1. ?s. (!a. P o a = TRUE <=> IN(a,s))”));
+
+
+(*
+ val it =
+   {},  |- !(a : mem(Pow(N0))). IN(a#, inN's) <=> SS(App(inNf, a#), a#): thm
+
+
+!a. IN(a,inN's) <=> SS(inNf o a,a)
+
+val fdef = FIf_def
+
+
+(*if use the same machinary as in SEAR, then for each f, need to invoke form2IL to build the predicate and prove the predicate has the desired property*)
+
+                         (
+qform2IL [‘s:1-> Exp(Exp(X,1+1),1+1)’] ‘!a.IN(a:1->Exp(X,1+1),f o s) ==> IN(a,s)’)
+*)
+fun mk_prim fdef = 
+    let val ((pname,psort),b) = fdef |> concl |> dest_forall
+        val ((mname,msort),b1) = b |> dest_forall
+        val pisin = psort|> dest_sort |> #2 |> el 2
+        val pvar = mk_var (pname,psort)
+       (* val fvar0 = mk_fvar "P" [mk_var (pname,psort)]*)
+        val (lb1,rb1) = b1 |> dest_dimp
+        val fnterm = lb1 |> dest_pred |> #2 |> el 2 |> dest_fun |> #3 |> hd
+       (* val fvar1 = mk_pred "SS" [mk_App fnterm pvar,pvar] *)
+        val defname = fnterm |> dest_fun |> #1 |> explode |> rev |> List.tl 
+                             |> rev |> implode
+        val spec_IN_ex = prim_lemma' |> sspecl [fnterm]
+                                    |> uex2ex_rule
+        val skinputs = cont spec_IN_ex 
+        val skinputs' = filter_cont skinputs |> HOLset.listItems
+        val sk = spec_IN_ex |> SKOLEM1 (defname ^ "'s") skinputs'
+    in sk
+    end
+
+
+
+fun mk_LFP primtm = 
+    let val bigintertm = mk_fun "BIGINTER" [primtm]
+        val defname = primtm |> dest_fun |> #1 |> explode |> rev |> tl |> tl
+                             |> rev |> implode
+        val st = sort_of bigintertm
+        val LFPname = defname^"s"
+        val templ = mk_eq (mk_var(defname^"s",st)) bigintertm
+        val exth = bigintertm |> refl 
+                              |> existsI (defname^"s",st) bigintertm templ
+        val skinputs = cont exth 
+        val skinputs' = filter_cont skinputs |> HOLset.listItems
+        val LFP_def = exth |> SKOLEM1 LFPname skinputs'
+    in LFP_def
+    end
+
+(*
+val LFPdef =  FIs_def
+val primdef = FI's_def
+
+*)
+
+
+fun mk_cond LFPdef primdef = 
+   let val avoids = HOLset.union(cont LFPdef,cont primdef)
+       val (LFP,bi) = LFPdef |> concl |> dest_eq
+       val pofset = bi |> sort_of
+                      |> #2 o dest_sort |> el 2 |> #3 o dest_fun |> hd
+       val memvar = pvariantt avoids (mk_var ("a",ar_sort ONE pofset))
+       val startwith = mk_pred "IN" [memvar,LFP]
+       val by_LFP = startwith |> basic_fconv (rewr_conv LFPdef)
+                              (rewr_fconv (spec_all IN_BIGINTER))
+       val by_primdef = by_LFP |> rewr_rule[primdef] |> GSYM
+       val gened = by_primdef |> allI (dest_var memvar)
+   in gened
+   end
+
+
+
+fun mk_SS LFPdef primdef = 
+    let val ((pname,psort),b) = primdef |> concl |> dest_forall
+        val s0 = psort |> dest_sort |> #2 |> el 2 |> dest_fun |> #3 |> hd
+        val (pl,pr) = b |> dest_dimp
+        val (LFP,bi) = LFPdef |> concl |> dest_eq
+        val pvar = mk_var (pname,psort)
+        val goal_conc = mk_pred "SS" [LFP,pvar]
+        val goal_ant = pr
+        val SS_bi = mk_pred "SS" [bi,pvar]
+        val by_LFP = goal_conc |> basic_fconv (rewr_conv LFPdef) no_fconv
+        val expand_SS = iff_trans by_LFP 
+                                  (SS_bi |> basic_fconv 
+                                   no_conv (rewr_fconv (spec_all SS_def))) 
+        val by_prim = expand_SS |> rewr_rule[IN_BIGINTER,primdef]
+                                |> iffRL |> undisch
+        val avoids = HOLset.union(cont LFPdef,cont primdef)
+        val genvar = pvariantt avoids (mk_var("a0",ar_sort ONE s0))
+        val lemmaf0 = mk_imp goal_ant (mk_pred "IN" [genvar,pvar]) 
+        val lemmaf = mk_forall pname psort lemmaf0
+        val lemma = lemmaf |> assume |> specl [pvar] 
+                           |> C mp (assume goal_ant)
+                           |> disch lemmaf
+                           |> allI (dest_var genvar)
+        val provedhyp = by_prim |> prove_hyp lemma
+        val disch_gen = provedhyp |> disch goal_ant |> allI (pname,psort)
+    in
+        disch_gen
+    end
+
+(*
+val monotone = FIf_monotone;
+val SS =  FIs_SS;
+val cond = FIs_cond; 
+*)
+
+fun mk_rules monotone SS cond = 
+    let val fnterm = monotone |> concl |> #1 o strip_forall
+                              |> #2 o dest_imp |> #2 o dest_pred
+                              |> hd |> #3 o dest_fun
+                              |> hd
+        val LFP = cond |> concl |> #1 o strip_forall
+                       |> #2 o dest_dimp |> #2 o dest_pred |> el 2
+        val st_genset = sort_of LFP
+        val LFP_in = st_genset |> (el 2) o #2 o dest_sort
+        val LFP_inpow = LFP_in |> hd o #3 o dest_fun
+        val avoids = HOLset.union(HOLset.union(cont monotone,cont SS),cont cond)
+        val genset = pvariantt avoids (mk_var ("s0",st_genset))
+        val fLFP = mk_App fnterm LFP
+        val th_stment = mk_pred "SS" [fLFP,genset]
+        val ori_goal = assume th_stment
+        val expand_SS0 = ori_goal |> rewr_rule[SS_def]
+        val ((memn,mems),_) = dest_forall (concl expand_SS0)
+        val expand_SS = expand_SS0 |> strip_all_and_imp
+        val itmd_set = mk_App fnterm genset
+        val spec_trans = SS_Trans |> specl [LFP_inpow,fLFP,itmd_set]
+                                  |> undisch
+                                  |> specl [genset]
+                                  |> undisch
+        val by_trans = expand_SS |> prove_hyp spec_trans
+        val spec_monotone = monotone |> specl [LFP,genset] |> undisch
+        val by_monotone = by_trans |> prove_hyp spec_monotone
+        val spec_SS = SS |> specl [genset] |> undisch
+        val by_SS = by_monotone |> prove_hyp spec_SS
+        val SS_assum = mk_pred "SS" [mk_App fnterm genset,genset]
+        val disch_SS_assum = by_SS |> disch SS_assum
+        val vgenset = dest_var genset
+        val by_cond = disch_SS_assum |> allI vgenset |> rewr_rule[cond]
+        val IN_assum = mk_pred "IN" [mk_var(memn,mems),fLFP] 
+        val disch_IN_assum = by_cond |> disch IN_assum
+        val wrap_SS = disch_IN_assum |> allI (memn,mems) |> rewr_rule[GSYM SS_def]
+    in wrap_SS
+    end
+
+(*
+val rules0 = FI_rules0
+val cond = FIs_cond
+*)
+
+fun mk_cases monotone rules0 cond = 
+    let val fLFP = rules0 |> concl |> #2 o dest_pred |> hd
+        val [fnterm,LFP] = fLFP |> #3 o dest_fun
+                           handle _ => raise 
+                                    simple_fail "mk_cases.cannot identify LFP"
+        val ((mname,msort),b) = cond |> concl |> dest_forall
+        val misin = msort |> dest_sort |> #2 |> el 2
+        val (lb,rb) = b |> dest_dimp
+        val ((sname,ssort),lb0) = lb |> dest_forall
+        val toasm_conseq = mk_pred "IN" [mk_var (mname,msort),fLFP]
+        val toasm_ant = mk_pred "SS" [mk_App fnterm fLFP,fLFP]
+        val orig = assume (mk_imp toasm_ant toasm_conseq)
+        val mp_ant = orig |> C mp (assume toasm_ant)
+        val spec_monotone = monotone |> specl [fLFP,LFP] |> undisch
+        val by_monotone = mp_ant |> prove_hyp spec_monotone
+        val by_rules0 = by_monotone |> prove_hyp rules0
+        val spec_asm_lb = lb |> assume |> specl [fLFP] 
+        val by_above = by_rules0 |> prove_hyp spec_asm_lb
+        val spec_cond = cond |> iffRL |> allE (mk_var (mname,msort)) |> undisch
+        val by_cond = by_above |> prove_hyp spec_cond |> disch rb
+                               |> allI (mname,msort)
+        val by_SS_def = by_cond |> rewr_rule[GSYM SS_def]
+        val conj = by_SS_def |> conjI rules0
+        val spec_SS_eq = SS_SS_eq |> specl [misin,fLFP,LFP]
+        val mp_above = conj |> mp spec_SS_eq
+    in mp_above
+    end
+
+fun mk_ind cond = 
+    let val ((memn,mems),b) = cond |> concl |> dest_forall
+        val toassume0 = b |> #1 o dest_dimp
+        val ((sname,ssort),toassume) = dest_forall toassume0
+        val tomp = toassume |> #1 o dest_imp
+        val orig = assume toassume
+        val mp_tomp = orig |> C mp (assume tomp)
+        val spec_toassume0 = toassume0 |> assume |> specl [mk_var (sname,ssort)]
+        val by_spec_above = mp_tomp |> prove_hyp spec_toassume0
+                                    |> disch toassume0
+                                    |> allI (memn,mems)
+        val by_cond = by_spec_above |> rewr_rule[cond]
+        val by_SS_def = by_cond |> rewr_rule[GSYM SS_def]
+        val disch_tomp = by_SS_def |> disch tomp
+        val gened = disch_tomp |> allI (sname,ssort)
+    in gened
+    end
+
+
+fun mk_Pow s = mk_fun "Exp" [s,TWO]
+
+                      
+(*have difficulty identify which is the input set on the RHS, so take a string x of its name, already know the sort should be the same as the output value set, so do not need to take a variable
+
+
+val inNf_ex =
+   {}, 
+   |- ?(f : fun(Pow(N0), Pow(N0))).
+        !(a : mem(Pow(N0)))  (n : mem(N0)).
+          IN(n#, App(f#, a#)) <=>
+          n# = O0 | ?(n0 : mem(N0)). IN(n0#, a#) & n# = App(S0, n0#): thm
+
+?FIf:Exp(Exp(X,2),2) -> Exp(Exp(X,2),2). 
+!xss:1-> Exp(Exp(X,2),2) xs:1->Exp(X,2).
+   IN(x,FIf o xs) <=> 
+   
+
+
+*)
+
+(*
+
+fun mk_fex incond x = 
+    let val ((mname,msort),b) = dest_forall incond
+        val mvar = mk_var(mname,msort)
+        val misin = msort |> dest_sort |> #2 |> hd
+        val powt = mk_Pow misin
+        val (lb,rb) = b |> dest_dimp 
+        val value_set = lb |> dest_pred |> #2 |> el 2
+        val valuest = sort_of value_set
+        val input_set = mk_var(x,valuest)
+        val tomp = IN_def_P_ex |> allE misin
+                            |> fVar_sInst_th (mk_fvar "P" [mvar]) rb
+                            |> allI (x,valuest)
+        val fvarP = mk_fvar "P" [input_set,value_set]
+        val spec_P2fun' = Rel2Ar' |> specl [powt,powt]
+                                 |> fVar_sInst_th fvarP incond
+        val mped = spec_P2fun' |> C mp tomp
+    in mped
+    end
+*)
+
+fun mk_fdef fname fexth = 
+    let val skinputs = (cont fexth) |> filter_cont |> HOLset.listItems 
+    in fexth |> SKOLEM1 fname skinputs
+    end
+
+fun mk_ind1 fdef ind0 = ind0 |> rewr_rule[SS_def,fdef]
+
+
+(*
+val fdef =  FIf_def;
+val cases0 = FI_cases0;
+*)
+
+(*IN_EXT_iff is only for N!!!!!*)
+
+fun mk_case1 fdef cases0 = 
+    let val (l,r) = dest_eq $ concl cases0
+        val spec_th = IN_EXT |> sspecl [l,r]
+        val app_spec_th = cases0 |> mp $ iffRL spec_th
+                                 |> rewr_rule[fdef]
+                                 |> GSYM
+    in app_spec_th
+    end
+
+fun mk_rules1 fdef rules0 = 
+    rules0 |> rewr_rule[SS_def,fdef]
+
+
+fun disj_imp_distr_fconv f = 
+    let val (ante,conseq) = dest_imp f
+        val (d1,d2) = dest_disj ante
+        val th0 = disj_imp_distr d1 d2 conseq
+    in th0
+    end
+
+(*
+
+(?(a : set). P(a#)) ==> Q(c) <=> 
+!a. P(a) ==> Q(c)
+
+rename due to:
+
+if (?a. P(a)) ==> Q(a)
+   then produce !a'. P(a') ==> Q(a) to avoid capture.
+
+val f = “(?a. P(a)) ==> Q(a)”
+*)
+
+fun pull_exists_fconv1 f = 
+    let val (ante,conseq) = dest_imp f 
+        val (v0 as (n,s),b) = dest_exists ante
+        val avoids = fvf f 
+        val vt = pvariantt avoids (mk_var v0)
+        val v = dest_var vt
+        val b' = substf (v0,vt) b
+        val goal = uncurry mk_forall v $ mk_imp b' conseq
+        val ex2all = b' |> assume |> existsI v0 vt b
+                        |> mp (assume f)
+                        |> disch b' |> allI v
+                        |> disch f
+        val all2ex = goal |> assume |> allE vt 
+                          |> undisch
+                          |> existsE v (assume ante)
+                          |> disch ante
+                          |> disch goal
+    in dimpI ex2all all2ex
+    end
+
+
+fun mk_rules2 rules1 = 
+    rules1 |> conv_rule
+              (basic_fconv no_conv disj_imp_distr_fconv)
+           |> conv_rule 
+              (basic_fconv no_conv pull_exists_fconv1)
+
+(*val f = “!a. P(a)& Q(a) ” “!a. P(a)& Q(a) <=> (!a.P(a)) & (!a.Q(a))” *)
+
+
+fun forall_conj_split_fconv f = 
+    let val (v as (n,s),c) = dest_forall f 
+        val (c1,c2) = dest_conj c 
+        val vt = mk_var v
+        val c1' = mk_forall n s c1 
+        val c2' = mk_forall n s c2 
+        val f' = mk_conj c1' c2' 
+        val l2r = conjI
+                      (f |> assume |> allE vt |> conjE1 
+                         |> allI v)
+                      (f |> assume |> allE vt |> conjE2
+                         |> allI v)
+                      |> disch f
+        val r2l = disch f' $ allI v $ conjI 
+                        (f' |> assume |> conjE1 |> allE vt)
+                        (f' |> assume |> conjE2 |> allE vt)
+    in dimpI l2r r2l
+    end
+
+
+fun exists_eq_fconv f = 
+    let val (v as (n,s),b) = dest_exists f
+        val (eqn,b0) = dest_conj b
+        val _ = is_eq eqn orelse 
+                raise ERR ("ex_eq_fconv.not an equation",[],[],[f])
+        val eqth = assume eqn
+        val b0th = basic_fconv (rewr_conv eqth) no_fconv b0
+        val b0th' = b0th |> iffLR |> undisch |> conj_assum eqn b0
+        val b0' = b0th |> concl |> dest_dimp |> #2
+        val l2r = existsE v (assume f) b0th' |> disch f
+        val (t1,t2) = dest_eq eqn
+        val th0 = conjI (refl t2) (assume b0')
+        val r2l = th0 |> existsI v t2 b |> disch b0'
+    in dimpI l2r r2l
+    end
+
+
+fun forall_eq_fconv f = 
+    let val (v as (n,s),b) = dest_forall f
+        val (eqn,conc) = dest_imp b
+        val (t1,t2) = dest_eq eqn
+        val l2r = assume f |> allE t2 |> C mp (refl t2) |> disch f
+        val eqth = sym (assume eqn)
+        val conc1 = substf (v,t2) conc
+        val r2l = assume conc1 |> rewr_rule[eqth] |> disch eqn |> allI v
+                         |> disch conc1
+    in dimpI l2r r2l
+    end
+
+
+fun conj_swap_fconv f = 
+    let val (p,q) = dest_conj f
+        val lhs = mk_conj p q
+        val rhs = mk_conj q p
+        val l2r = conjI (assume lhs |> conjE2) (assume lhs |> conjE1) 
+                        |> disch lhs
+        val r2l = conjI (assume rhs |> conjE2) (assume rhs |> conjE1) 
+                        |> disch rhs
+    in
+        dimpI l2r r2l
+    end
+
+fun conj_assoc_fconv f =
+    let val (AB,C) = dest_conj f
+        val (A,B) = dest_conj AB
+        val AB = mk_conj A B
+        val BC = mk_conj B C
+        val ABC1 = mk_conj AB C
+        val ABC = mk_conj A BC
+        val l2r = conjI (assume ABC1 |> conjE1 |> conjE1)
+                        (conjI (assume ABC1 |> conjE1 |> conjE2)
+                               (assume ABC1 |> conjE2)) |> disch_all
+        val r2l = conjI (conjI (assume ABC |> conjE1)
+                               (assume ABC |> conjE2 |> conjE1))
+                        (assume ABC |> conjE2 |> conjE2) |> disch_all
+    in 
+        dimpI l2r r2l
+    end
+
+
+
+fun conj_cossa_fconv f =
+    let val (A,BC) = dest_conj f
+        val (B,C) = dest_conj BC
+        val AB = mk_conj A B
+        val BC = mk_conj B C
+        val ABC1 = mk_conj AB C
+        val ABC = mk_conj A BC
+        val l2r = conjI (assume ABC1 |> conjE1 |> conjE1)
+                        (conjI (assume ABC1 |> conjE1 |> conjE2)
+                               (assume ABC1 |> conjE2)) |> disch_all
+        val r2l = conjI (conjI (assume ABC |> conjE1)
+                               (assume ABC |> conjE2 |> conjE1))
+                        (assume ABC |> conjE2 |> conjE2) |> disch_all
+    in 
+        dimpI r2l l2r
+    end
+
+
+fun PULL_CONJ p f = 
+  if p f then SOME (frefl f)
+  else
+    case view_form f of
+      vConn("&", [f1,f2]) => 
+       (case (PULL_CONJ p) f1 of
+          NONE => (case (PULL_CONJ p) f2 of
+                     NONE => NONE
+                   | SOME f2eqth => 
+                     if is_eq (f2eqth |> concl |> dest_dimp |> #2)
+                     then 
+                         let val th1 = conj_iff (frefl f1) f2eqth
+                             val f0 = mk_conj f1 (f2eqth |> concl |> dest_dimp |> #2)
+                             val f0th = conj_swap_fconv f0
+                         in SOME (iff_trans th1 f0th)
+                         end
+                     else
+                     let val eqandsth = f2eqth |> concl |> dest_dimp |> #2
+                         val f2eqth' = iff_trans f2eqth (conj_swap_fconv eqandsth)
+                         val cth = conj_iff (frefl f1) f2eqth'
+                         val tocossa = cth |> concl |> dest_dimp |> #2
+                         val th' = tocossa |> (conj_cossa_fconv thenfc conj_swap_fconv)
+                         val th1 = iff_trans cth th'
+                     in SOME th1
+                     end)
+        | SOME f1eqth => 
+          let val th0 = conj_iff f1eqth (frefl f2) 
+              val f' = th0 |> concl |> dest_dimp |> #2
+          in
+          SOME (iff_trans th0 (try_fconv conj_assoc_fconv f'))
+          end)
+    | _ => NONE
+
+fun pull_conj_fconv p f = 
+    case PULL_CONJ p f of SOME th => th
+                      | _ => raise simple_fail "pull_conj_fconv";
+
+
+
+fun conj_imp_fconv f = 
+    let 
+        val (AB,C) = dest_imp f
+        val (A,B) = dest_conj AB
+        val ab = mk_conj A B
+        val ab2c = mk_imp ab C
+        val a2b2c = mk_imp A (mk_imp B C)
+        val conjabonc = mp (assume ab2c) (conjI (assume A) (assume B))
+        val conj2imp = disch ab2c (disch A (disch B conjabonc))
+        val abona = conjE1 (assume ab)
+        val abonb = conjE2 (assume ab)
+        val imp2conj = disch a2b2c (disch ab (mp (mp (assume a2b2c) abona) abonb))
+    in dimpI conj2imp imp2conj
+    end
+
+(*--find among the conjunctions if there is a equation,
+  --if there is one, then pull it out to the outmost conj
+  --fconv into a = b ==> ... to apply forall_eq_fconv
+  --quantifier order *)
+
+
+
+
+fun remove_list_item i l = 
+    case l of [] => []
+            | h :: t => 
+              if (h = i) then t else
+              h :: (remove_list_item  i t)
+
+fun mk_foralls vl f = 
+    case vl of [] => f 
+             | h :: t => uncurry mk_forall h (mk_foralls t f)
+
+fun forall_in_eq_fconv f = 
+    let val (b,vs) = strip_forall f
+        val (ante,conc) = dest_imp b 
+        val (l,r) = dest_eq ante 
+        val v = dest_var l
+        val vs' = remove_list_item v vs
+        val vl = (rev $ v :: rev vs')
+        val f' = mk_foralls vl b
+        val l2r = f |> assume |> specl (List.map mk_var vs)
+                    |> simple_genl vl |> disch f
+        val r2l = f'|> assume |> specl (List.map mk_var vl)
+                    |> simple_genl vs |> disch f'
+    in dimpI l2r r2l
+    end
+
+
+fun mk_rules3 rules2 = 
+rules2  |> conv_rule (basic_fconv no_conv forall_conj_split_fconv)
+  |> conv_rule (basic_fconv no_conv forall_eq_fconv)
+  |> conv_rule (basic_once_fconv no_conv (pull_conj_fconv is_eq))
+  |> conv_rule (basic_fconv no_conv conj_imp_fconv) 
+  |> conv_rule (basic_once_fconv no_conv forall_in_eq_fconv)
+  (*do not understand why forall_in_eq_fconv can loop*)
+  |> conv_rule (basic_fconv no_conv forall_eq_fconv)
+
+(*A ==> C & B ==> C <=> A | B ==> C*)
+
+fun disj_imp_undistr_fconv f = 
+    let val (imp1,imp2) = dest_conj f 
+        val (A,C1) = dest_imp imp1 
+        val (B,C2) = dest_imp imp2 
+        val _ = eq_form(C1,C2) orelse raise ERR ("disj_imp_undistr_fconv.conclusion not same",[],[],[C1,C2]) 
+        val th0 = disj_imp_distr A B C1
+    in GSYM th0 
+    end
+
+
+(*“!a.P(a) ==> Q” *)
+fun unpull_exists_fconv1 f = 
+    let val (v as (n,s),b) = dest_forall f 
+        val (ante,conc) = dest_imp b
+        val vt = mk_var v
+        val eante = (uncurry mk_exists v ante)
+        val goal = mk_imp eante conc
+        val ex2all = ante |> assume |> existsI v vt ante
+                          |> mp (assume goal)
+                          |> disch ante |> allI v
+                          |> disch goal
+        val all2ex = f |> assume |> allE vt 
+                       |> undisch
+                       |> existsE v (assume eante)
+                       |> disch eante
+                       |> disch f
+    in dimpI all2ex ex2all 
+    end
+
+(*
+val f = “(n = O0 ==> IN(n,inN)) &
+         (!n0. IN(n0,inN) & n = App(S1,n0) ==> IN(n,inN))”
+
+val f = “(xs = Empty(X) ==> IN(xs,FI)) &
+         (!xs0:mem(Pow(X)) x. IN(xs0,FI) & xs = Ins(x,xs0) ==>
+         IN(xs,FI))”
+
+val f = “(xsn = Pair(Empty(X),O) ==> IN(xsn,Cd)) &
+         (!xsn0 x. IN(xsn0,Cd) &  ~(IN(x,Fst(xsn0))) & 
+          xsn = Pair(Ins(x,Fst(xsn0)),Suc(Snd(xsn0))) ==>
+         IN(xsn,Cd))”
+
+val f = “(ls = Empty(N * X) ==> IN(ls,isL)) &
+         (!ls0 x. IN(ls0,isL) & ls = Ins(Pair(CARD(ls0),x),ls0) ==> IN(ls,isL)) ”
+*)
+(*
+unpull_exists_fconv1 “(!n0. IN(n0,inN) & n = App(S1,n0) ==> IN(n,inN))”
+*)
+
+fun mk_incond f = 
+    let val th0 = basic_fconv no_conv unpull_exists_fconv1 f
+        (*ideally, will give identical conclusion*)
+        val f1 = th0 |> concl |> dest_dimp |> #2
+        val th1 = basic_fconv no_conv disj_imp_undistr_fconv f1
+        val f2 = th1 |> concl |> dest_dimp |> #2
+        val (ante,conc) = dest_imp f2
+        val [qv,newtm] = conc |> dest_pred |> #2
+        val (newname,st) = dest_var newtm
+        (*check avoids here*)
+        val fiv = mk_var (newname ^ "0",st) 
+        val fov = mk_var (newname ^ "1",st)
+        val conc' = substf ((newname,st),fov) conc
+        val ante' = substf ((newname,st),fiv) ante
+        val f3 = uncurry mk_forall (dest_var qv) 
+                         (mk_dimp conc' ante')
+    in (f3,newname ^ "0")
+    end
+
+(*
+
+basic_once_fconv to use is_eq not good, will try write this
+
+fun all_conj_fconv fc = 
+    let val 
+
+*)
+
+fun mk_ind2 ind1 = 
+    ind1 |> conv_rule 
+         (basic_fconv no_conv disj_imp_distr_fconv)
+         |> conv_rule 
+         (basic_fconv no_conv forall_conj_split_fconv)
+         |> conv_rule 
+         (basic_fconv no_conv pull_exists_fconv1) 
+         |> conv_rule
+         (basic_once_fconv no_conv (pull_conj_fconv is_eq))
+         (*want to use once rather then basic since the eqn if exists musst be the first one, bu seems not sufficient, a conv only apply once until success?*)
+         |> conv_rule
+         (basic_fconv no_conv conj_imp_fconv)
+         |> conv_rule
+         (basic_once_fconv no_conv forall_in_eq_fconv)
+         |> conv_rule
+         (basic_once_fconv no_conv forall_eq_fconv)
+         |> conv_rule
+         (basic_fconv no_conv (rewr_fconv $ GSYM CONJ_IMP_IMP))
+
+
+(*
+
+
+val FI_cl = 
+ “(xs = Empty(X) ==> IN(xs,FIs)) &
+  (!xs0 x. IN(xs0,FIs) & xs = Ins(x,xs0) ==> IN(xs,FIs))”
+
+
+
+val inN_cl = 
+ “(n = O0 ==> IN(n,inN)) &
+  (!n0. IN(n0,inN) & n = S0 o n0 ==> IN(n,inN))”
+
+
+
+val (inN_incond,x1) = mk_incond inN_cl;
+val inNf_ex = mk_fex inN_incond x1;
+val inNf_def = mk_fdef "inNf" inNf_ex;
+val inNf_monotone = mk_monotone inNf_def;
+val inN's_def = mk_prim inNf_def;
+val inNs_def = mk_LFP (rastt "inN's");
+val inNs_cond = mk_cond inNs_def inN's_def;
+val inNs_SS = mk_SS inNs_def inN's_def;
+val inN_rules0 = mk_rules inNf_monotone inNs_SS inNs_cond;
+val inN_cases0 = mk_cases inNf_monotone inN_rules0 inNs_cond;
+val inN_ind0 = mk_ind inNs_cond;
+val inN_ind1 = mk_ind1 inNf_def inN_ind0;
+val inN_ind2 = mk_ind2 inN_ind1;
+val inN_cases1 = mk_case1 inNf_def inN_cases0;
+val inN_rules1 = mk_rules1 inNf_def inN_rules0;
+val inN_rules2 = mk_rules2 inN_rules1;
+val inN_rules3 = mk_rules3 inN_rules2;
+
+> val inN_incond =
+   !(n : mem(N0)).
+     IN(n#, inN1) <=>
+     n# = O0 | ?(n0 : mem(N0)). IN(n0#, inN0) & n# = App(S0, n0#): form
+val x1 = "inN0": string
+val inNf_ex =
+   {}, 
+   |- ?(f : fun(Pow(N0), Pow(N0))).
+        !(a : mem(Pow(N0)))  (n : mem(N0)).
+          IN(n#, App(f#, a#)) <=>
+          n# = O0 | ?(n0 : mem(N0)). IN(n0#, a#) & n# = App(S0, n0#): thm
+val inNf_def =
+   {}, 
+   |- !(a : mem(Pow(N0)))  (n : mem(N0)).
+        IN(n#, App(inNf, a#)) <=>
+        n# = O0 | ?(n0 : mem(N0)). IN(n0#, a#) & n# = App(S0, n0#): thm
+val inNf_monotone =
+   {}, 
+   |- !(s1 : mem(Pow(N0)))  (s2 : mem(Pow(N0))).
+        SS(s1#, s2#) ==> SS(App(inNf, s1#), App(inNf, s2#)): thm
+val inN's_def =
+   {},  |- !(a : mem(Pow(N0))). IN(a#, inN's) <=> SS(App(inNf, a#), a#): thm
+val inNs_def = {},  |- inNs = BIGINTER(inN's): thm
+val inNs_cond =
+   {}, 
+   |- !(a : mem(N0)).
+        (!(ss : mem(Pow(N0))). SS(App(inNf, ss#), ss#) ==> IN(a#, ss#)) <=>
+        IN(a#, inNs): thm
+val inNs_SS =
+   {},  |- !(a : mem(Pow(N0))). SS(App(inNf, a#), a#) ==> SS(inNs, a#): thm
+val inN_rules0 = {},  |- SS(App(inNf, inNs), inNs): thm
+val inN_cases0 = {},  |- App(inNf, inNs) = inNs: thm
+val inN_ind0 =
+   {},  |- !(ss : mem(Pow(N0))). SS(App(inNf, ss#), ss#) ==> SS(inNs, ss#):
+   thm
+val inN_ind1 =
+   {}, 
+   |- !(ss : mem(Pow(N0))).
+        (!(a : mem(N0)).
+            a# = O0 | (?(n0 : mem(N0)). IN(n0#, ss#) & a# = App(S0, n0#)) ==>
+            IN(a#, ss#)) ==> !(a : mem(N0)). IN(a#, inNs) ==> IN(a#, ss#):
+   thm
+val inN_ind2 =
+   {}, 
+   |- !(ss : mem(Pow(N0))).
+        IN(O0, ss#) &
+        (!(n0 : mem(N0)). IN(n0#, ss#) ==> IN(App(S0, n0#), ss#)) ==>
+        !(a : mem(N0)). IN(a#, inNs) ==> IN(a#, ss#): thm
+val inN_cases1 =
+   {}, 
+   |- !(x : mem(N0)).
+        IN(x#, inNs) <=>
+        x# = O0 | ?(n0 : mem(N0)). IN(n0#, inNs) & x# = App(S0, n0#): thm
+val inN_rules1 =
+   {}, 
+   |- !(a : mem(N0)).
+        a# = O0 | (?(n0 : mem(N0)). IN(n0#, inNs) & a# = App(S0, n0#)) ==>
+        IN(a#, inNs): thm
+val inN_rules2 =
+   {}, 
+   |- !(a : mem(N0)).
+        (a# = O0 ==> IN(a#, inNs)) &
+        !(n0 : mem(N0)). IN(n0#, inNs) & a# = App(S0, n0#) ==> IN(a#, inNs):
+   thm
+val inN_rules3 =
+   {}, 
+   |- IN(O0, inNs) &
+      !(n0 : mem(N0)). IN(n0#, inNs) ==> IN(App(S0, n0#), inNs): thm
+
+
+> # # # val inN_ind =
+   {}, 
+   |- !(ss : mem(Pow(N0))).
+        IN(O0, ss#) &
+        (!(n0 : mem(N0)). IN(n0#, ss#) ==> IN(App(S0, n0#), ss#)) ==>
+        !(a : mem(N0)). IN(a#, inNs) ==> IN(a#, ss#): thm
+> val inN_cases =
+   {}, 
+   |- !(x : mem(N0)).
+        IN(x#, inNs) <=>
+        x# = O0 | ?(n0 : mem(N0)). IN(n0#, inNs) & x# = App(S0, n0#): thm
+> val inN_rules =
+   {}, 
+   |- IN(O0, inNs) &
+      !(n0 : mem(N0)). IN(n0#, inNs) ==> IN(App(S0, n0#), inNs): thm
+ val FIf_def =
+   {(X : set)}, 
+   |- !(a : mem(Pow(Pow(X))))  (xs : mem(Pow(X))).
+        IN(xs#, App(FIf(X), a#)) <=>
+        xs# = Empty(X) |
+        ?(xs0 : mem(Pow(X)))  (x : mem(X)).
+          IN(xs0#, a#) & xs# = Ins(x#, xs0#): thm
+
+
+
+ex
+{(X : set)}, 
+   |- ?(f : fun(Pow(Pow(X)), Pow(Pow(X)))).
+        !(a : mem(Pow(Pow(X))))  (xs : mem(Pow(X))).
+          IN(xs#, App(f#, a#)) <=>
+          xs# = Empty(X) |
+          ?(xs0 : mem(Pow(X)))  (x : mem(X)).
+            IN(xs0#, a#) & xs# = Ins(x#, xs0#): thm
+
+
+val it =
+   (!(xs : mem(Pow(X))).
+      IN(xs#, FIs1) <=>
+      xs# = Empty(X) |
+      ?(xs0 : mem(Pow(X)))  (x : mem(X)).
+        IN(xs0#, FIs0) & xs# = Ins(x#, xs0#), "Lind0")
+
+val FIf_monotone =
+   {(X : set)}, 
+   |- !(s1 : mem(Pow(Pow(X))))  (s2 : mem(Pow(Pow(X)))).
+        SS(s1#, s2#) ==> SS(App(FIf(X), s1#), App(FIf(X), s2#)): thm
+val FI's_def =
+   {(X : set)}, 
+   |- !(a : mem(Pow(Pow(X)))). IN(a#, FI's(X)) <=> SS(App(FIf(X), a#), a#):
+   thm
+val FIs_def = {(X : set)},  |- FIs(X) = BIGINTER(FI's(X)): thm
+val FIs_cond =
+   {(X : set)}, 
+   |- !(a : mem(Pow(X))).
+        (!(ss : mem(Pow(Pow(X)))). SS(App(FIf(X), ss#), ss#) ==> IN(a#, ss#)) <=>
+        IN(a#, FIs(X)): thm
+val FIs_SS =
+   {(X : set)}, 
+   |- !(a : mem(Pow(Pow(X)))). SS(App(FIf(X), a#), a#) ==> SS(FIs(X), a#):
+   thm
+val FI_rules0 = {(X : set)},  |- SS(App(FIf(X), FIs(X)), FIs(X)): thm
+val FI_cases0 = {(X : set)},  |- App(FIf(X), FIs(X)) = FIs(X): thm
+val FI_ind0 =
+   {(X : set)}, 
+   |- !(ss : mem(Pow(Pow(X)))). SS(App(FIf(X), ss#), ss#) ==> SS(FIs(X), ss#):
+   thm
+val FI_ind1 =
+   {(X : set)}, 
+   |- !(ss : mem(Pow(Pow(X)))).
+        (!(a : mem(Pow(X))).
+            a# = Empty(X) |
+            (?(xs0 : mem(Pow(X)))  (x : mem(X)).
+                IN(xs0#, ss#) & a# = Ins(x#, xs0#)) ==> IN(a#, ss#)) ==>
+        !(a : mem(Pow(X))). IN(a#, FIs(X)) ==> IN(a#, ss#): thm
+val FI_ind2 =
+   {(X : set)}, 
+   |- !(ss : mem(Pow(Pow(X)))).
+        IN(Empty(X), ss#) &
+        (!(xs0 : mem(Pow(X)))  (x : mem(X)).
+            IN(xs0#, ss#) ==> IN(Ins(x#, xs0#), ss#)) ==>
+        !(a : mem(Pow(X))). IN(a#, FIs(X)) ==> IN(a#, ss#): thm
+val FI_cases1 =
+   {(X : set)}, 
+   |- !(x : mem(Pow(X))).
+        IN(x#, FIs(X)) <=>
+        x# = Empty(X) |
+        ?(xs0 : mem(Pow(X)))  (x : mem(X)).
+          IN(xs0#, FIs(X)) & x# = Ins(x#, xs0#): thm
+val FI_rules1 =
+   {(X : set)}, 
+   |- !(a : mem(Pow(X))).
+        a# = Empty(X) |
+        (?(xs0 : mem(Pow(X)))  (x : mem(X)).
+            IN(xs0#, FIs(X)) & a# = Ins(x#, xs0#)) ==> IN(a#, FIs(X)): thm
+val FI_rules2 =
+   {(X : set)}, 
+   |- !(a : mem(Pow(X))).
+        (a# = Empty(X) ==> IN(a#, FIs(X))) &
+        !(xs0 : mem(Pow(X)))  (x : mem(X)).
+          IN(xs0#, FIs(X)) & a# = Ins(x#, xs0#) ==> IN(a#, FIs(X)): thm
+val FI_rules3 =
+   {(X : set)}, 
+   |- IN(Empty(X), FIs(X)) &
+      !(xs0 : mem(Pow(X)))  (x : mem(X)).
+        IN(xs0#, FIs(X)) ==> IN(Ins(x#, xs0#), FIs(X)): thm
+val it = (): unit
+*)
